@prefix rdf: <http://www.w3.org/1999/02/22-rdf-syntax-ns#> .
@prefix rdfs: <http://www.w3.org/2000/01/rdf-schema#> .
@prefix skos: <http://www.w3.org/2004/02/skos/core#> .
@prefix dcterms: <http://purl.org/dc/terms/> .
@prefix vfm: <http://gridappsd.org/variable-fidelity#> .

# VFM Concept Scheme
<http://gridappsd.org/variable-fidelity/concepts> a skos:ConceptScheme ;
    dcterms:title "Variable Fidelity Modeling Concepts" ;
    dcterms:description "Conceptual classification for variable fidelity grid model data" ;
    dcterms:creator "UCAiUG CIM Users Group" ;
    vfm:supportsFidelityLevels vfm:HighFidelity, vfm:MediumFidelity, vfm:LowFidelity .

# Model Type Concepts
vfm:ConnectivityModel a skos:Concept ;
    skos:inScheme <http://gridappsd.org/variable-fidelity/concepts> ;
    skos:prefLabel "Connectivity Model" ;
    skos:definition "Model data describing equipment connectivity and topology" ;
    skos:topConceptOf <http://gridappsd.org/variable-fidelity/concepts> ;
    vfm:requiredForFidelity vfm:LowFidelity, vfm:MediumFidelity, vfm:HighFidelity .

vfm:GeographicalModel a skos:Concept ;
    skos:inScheme <http://gridappsd.org/variable-fidelity/concepts> ;
    skos:prefLabel "Geographical Model" ;
    skos:definition "Model data describing geographical location and spatial relationships" ;
    skos:topConceptOf <http://gridappsd.org/variable-fidelity/concepts> ;
    vfm:requiredForFidelity vfm:MediumFidelity, vfm:HighFidelity .

vfm:ElectricalModel a skos:Concept ;
    skos:inScheme <http://gridappsd.org/variable-fidelity/concepts> ;
    skos:prefLabel "Electrical Model" ;
    skos:definition "Model data describing electrical characteristics and parameters" ;
    skos:topConceptOf <http://gridappsd.org/variable-fidelity/concepts> ;
    vfm:requiredForFidelity vfm:HighFidelity .

# Export Control Concepts
vfm:ExportControlModel a skos:Concept ;
    skos:inScheme <http://gridappsd.org/variable-fidelity/concepts> ;
    skos:prefLabel "Export Control Model" ;
    skos:definition "Rules and policies governing data export based on fidelity requirements" ;
    skos:topConceptOf <http://gridappsd.org/variable-fidelity/concepts> .

# Fidelity-specific subconcepts
vfm:HighFidelityTopology a skos:Concept ;
    skos:inScheme <http://gridappsd.org/variable-fidelity/concepts> ;
    skos:prefLabel "High Fidelity Topology" ;
    skos:broader vfm:ConnectivityModel ;
    skos:definition "Detailed connectivity model with all switching devices and connection points" .

vfm:SimplifiedTopology a skos:Concept ;
    skos:inScheme <http://gridappsd.org/variable-fidelity/concepts> ;
    skos:prefLabel "Simplified Topology" ;
    skos:broader vfm:ConnectivityModel ;
    skos:definition "Simplified connectivity model focusing on major equipment only" .